Main.lean
@@ -3,6 +3,6 @@ import HexLuthor
 open HexLuthor
 
 def main : IO Unit := do
-  IO.println s!"White: {Hex.toHexString #h"FFFFFF"}"
-  IO.println s!"Red: {Hex.toHexString #h"FF0000"}"
-  IO.println s!"Royal Blue: {Hex.toHexString #h"4169E1"}"
+  IO.println s!"White: {Hex.toHexString #xFFFFFF}"
+  IO.println s!"Red: {Hex.toHexString #xFF0000}"
+  IO.println s!"Royal Blue: {Hex.toHexString #x4169E1}"
